src/kemedhoc/Impl.KEMEDHOC.Core.Msg1.fst
@@ -1,0 +1,165 @@
+module Impl.KEMEDHOC.Core.Msg1
+
+(*HACL Random lib*)
+open Lib.RandomBuffer.System
+
+module B = LowStar.Buffer
+module ST = FStar.HyperStack.ST
+module HS = FStar.HyperStack
+module S = FStar.Seq
+module Seq = Lib.Sequence
+
+module FBytes = FStar.Bytes
+
+(*Specification modules*)
+module Spec = Spec.KEMEDHOC.Core
+friend Spec.KEMEDHOC.Core
+
+module SpecCrypto = Spec.KEMEDHOC.CryptoPrimitives
+module SpecParser = Spec.KEMEDHOC.Parser
+
+module TypeEdhoc = TypeHelper.EDHOC
+module SpecEdhocSerd = Spec.EDHOC.Serialization
+
+#push-options "--z3rlimit 60 --max_fuel 4 --max_ifuel 4"
+let initiator_send_msg1 kcs is msg1 hs
+  = ST.push_frame();
+  (**) let h0 = ST.get () in
+
+  // generate connection ID C_I
+  crypto_random msg1.c_i (size SpecParser.c_id_size);
+  (**) let h1 = ST.get () in
+  (**) assert(modifies (loc entropy_p |+| loc msg1.c_i) h0 h1);
+
+  // generate ephemeral KEM key pair
+  let pk_x = msg1.pk_x in
+  let sk_x = is.eph_kem_priv_key.value in
+  let sk_x_is_some = is.eph_kem_priv_key.is_some in
+  (**) assert(disjoint pk_x sk_x);
+  kem_keygen kcs pk_x sk_x;
+  (**) let h2 = ST.get () in
+  (**) assert(modifies (loc entropy_p |+| loc msg1.c_i
+            |+| loc pk_x |+| loc sk_x |+| loc kem_state
+  ) h0 h2);
+  nat_to_bytes 1ul sk_x_is_some 1;
+  (**) let h2_1 = ST.get () in
+  (**) assert(modifies1 sk_x_is_some h2 h2_1);
+  (**) assert(modifies (loc entropy_p |+| loc msg1.c_i
+            |+| loc pk_x |+| loc sk_x |+| loc kem_state
+            |+| loc sk_x_is_some
+  ) h0 h2);
+
+  // encap the Responder's static public KEM key for authentication
+  let ct_auth_R = msg1.ct_auth_R in
+  let k_auth_R = hs.k_auth_R in
+  (**) assert(B.all_disjoint [loc is.remote_static_kem_pub_key; loc ct_auth_R; loc k_auth_R; loc entropy_p; loc kem_state]);
+  kem_encaps kcs is.remote_static_kem_pub_key ct_auth_R k_auth_R;
+  (**) let h3 = ST.get () in
+  // (**) assert(modifies (loc entropy_p |+| loc kem_state |+| loc ct_auth_R
+  //                     |+| loc k_auth_R) h0 h3);
+  (**) assert(modifies (loc entropy_p |+| loc msg1.c_i
+            |+| loc pk_x |+| loc sk_x |+| loc kem_state
+            |+| loc sk_x_is_some
+            |+| loc ct_auth_R |+| loc k_auth_R
+  ) h0 h3);
+
+  // compute TH1
+  compute_th1 #kcs pk_x ct_auth_R hs.th1;
+  (**) let h4 = ST.get () in
+  (**) assert(modifies1 hs.th1 h3 h4);
+  (**) assert( modifies (loc entropy_p |+| loc msg1.c_i
+            |+| loc pk_x |+| loc sk_x |+| loc kem_state
+            |+| loc sk_x_is_some
+            |+| loc ct_auth_R |+| loc k_auth_R
+            |+| loc hs.th1
+  ) h0 h4);
+
+  // derive PRK1e
+  extract_prk1e #kcs hs.th1 k_auth_R hs.prk1e;
+  (**) let h5 = ST.get () in
+  (**) assert(modifies1 hs.prk1e h4 h5);
+  (**) assert( modifies (loc entropy_p |+| loc msg1.c_i
+            |+| loc pk_x |+| loc sk_x |+| loc kem_state
+            |+| loc sk_x_is_some
+            |+| loc ct_auth_R |+| loc k_auth_R
+            |+| loc hs.th1
+            |+| loc hs.prk1e
+  ) h0 h5);
+
+  // construct credential payload
+  let cred_I = create (size SpecParser.cred_size) (u8 0) in
+  copy cred_I is.id_cred;
+  (**) let h6 = ST.get () in
+  // (**) assert(modifies1 cred_I h5 h6);
+  (**) assert(modifies (loc entropy_p |+| loc msg1.c_i
+            |+| loc pk_x |+| loc sk_x |+| loc kem_state
+            |+| loc sk_x_is_some
+            |+| loc ct_auth_R |+| loc k_auth_R
+            |+| loc hs.th1
+            |+| loc hs.prk1e
+            |+| loc cred_I)
+  h0 h6);
+
+  // construct plaintext1
+  let p1 = construct_plaintext1 is.id_cred cred_I in
+  let ptx1_concat_len = plaintext1_size_t in
+  (**) assert(is_valid_plaintext1 h6 p1);
+
+  // encrypt plaintext1 to ciphertext1
+  let res = encrypt_plaintext1 #kcs p1 hs.th1 hs.prk1e msg1.c1 in
+  (**) let h7 = ST.get () in
+  (**) assert(match res with
+    | TypeEdhoc.CUnsupportedAlgorithmOrInvalidConfig | TypeEdhoc.CSuccess -> True
+    | _ -> False  
+  );
+
+  let final_res = match res with
+    | TypeEdhoc.CUnsupportedAlgorithmOrInvalidConfig -> (
+      (**) assert(modifies0 h6 h7);
+      (**) assert(modifies (loc entropy_p |+| loc msg1.c_i
+            |+| loc pk_x |+| loc sk_x |+| loc kem_state
+            |+| loc sk_x_is_some
+            |+| loc ct_auth_R |+| loc k_auth_R
+            |+| loc hs.th1
+            |+| loc hs.prk1e
+            |+| loc cred_I
+      ) h0 h7);
+      res
+    )
+    | TypeEdhoc.CSuccess -> (
+      (**) let hx = ST.get() in
+      (**) assert(TypeEdhoc.CSuccess? res);
+      // (**) assert(modifies1 msg1.c1 h6 h7);
+      // construct message1
+      // only need to update the method and suite_i fields
+      (**) assert(live hx msg1.method /\ FBytes.repr_bytes 5 = 1);
+      nat_to_bytes 1ul msg1.method 5;
+      let suite_label = Some?.v (SpecCrypto.get_kemCipherSuite_label kcs) in
+      (**) assert(live hx msg1.suite_i /\ FBytes.repr_bytes suite_label = 1);
+      nat_to_bytes 1ul msg1.suite_i suite_label;
+      (**) let h8 = ST.get () in
+      (**) assert(
+        SpecEdhocSerd.bytes_to_nat (as_seq h8 msg1.method) = 5
+        /\ SpecEdhocSerd.bytes_to_nat (as_seq h8 msg1.suite_i) = Some?.v (SpecCrypto.get_kemCipherSuite_label kcs)
+      );
+
+      // compute hash of message1
+      let msg1_concat_len = concat_msg1_fixed_length_t kcs in
+      let msg1_concat_buffer = create msg1_concat_len (u8 0) in
+      (**) assert(message1_disjoint_to_lbuffer msg1 msg1_concat_buffer);
+      (**) assert(is_valid_message1 h8 msg1);
+      concat_msg1 kcs msg1 msg1_concat_buffer;
+      (**) let h9 = ST.get () in
+
+      (**) assert(disjoint msg1_concat_buffer hs.msg1_hash);
+      (**) assert(live h9 msg1_concat_buffer /\ live h9 hs.msg1_hash);
+      do_hash kcs hs.msg1_hash msg1_concat_len msg1_concat_buffer;
+      (**) let h10 = ST.get () in
+
+      res 
+    ) in
+
+    ST.pop_frame();
+    final_res
+
+#pop-options
