src/kemedhoc/Impl.KEMEDHOC.Core.Msg1.fsti
@@ -1,0 +1,78 @@
+module Impl.KEMEDHOC.Core.Msg1
+
+(*LowStar related modules*)
+open Lib.ByteBuffer
+open Lib.IntTypes
+open Lib.Buffer
+
+(*HACL Random lib*)
+open Lib.RandomBuffer.System
+
+module B = LowStar.Buffer
+module ST = FStar.HyperStack.ST
+module HS = FStar.HyperStack
+module S = FStar.Seq
+module Seq = Lib.Sequence
+
+(*Specification modules*)
+module Spec = Spec.KEMEDHOC.Core
+
+module SpecCrypto = Spec.KEMEDHOC.CryptoPrimitives
+module SpecParser = Spec.KEMEDHOC.Parser
+
+module TypeEdhoc = TypeHelper.EDHOC
+
+(*EDHOC utilities*)
+open Impl.EDHOC.Utilities
+
+(*KEMEDHOC utilities*)
+open Impl.KEMEDHOC.Types
+open Impl.KEMEDHOC.CryptoPrimitives
+open Impl.KEMEDHOC.KeySchedule
+open Impl.KEMEDHOC.Parser
+open Impl.KEMEDHOC.Ciphertext
+open Impl.KEMEDHOC.TranscriptHash
+open Impl.KEMEDHOC.Core
+open Spec.KEMEDHOC.Base.Definitions
+
+(*------------------ Message 1*)
+val initiator_send_msg1:
+  kcs: supportedKemCipherSuite
+  -> is: party_state_m kcs
+  -> msg1: message1 kcs
+  -> hs: handshake_state_m kcs
+  -> ST.Stack c_response
+  (requires fun h0 ->
+    is_valid_party_state_m h0 is /\ live h0 entropy_p /\ live h0 kem_state
+    /\ is_valid_handshake_state_m h0 hs /\ is_valid_message1 h0 msg1
+    
+    // Disjointness
+    /\ handshake_state_m_disjoint_to_party_state hs is
+    /\ handshake_state_m_disjoint_to_lbuffer hs kem_state
+    /\ handshake_state_m_disjoint_to_lbuffer hs entropy_p
+    /\ handshake_state_m_disjoint_to_msg1 hs msg1
+    /\ party_state_disjoint_to_lbuffer is kem_state
+    /\ party_state_disjoint_to_lbuffer is entropy_p
+    /\ party_state_disjoint_to_msg1 is msg1
+    /\ message1_disjoint_to_lbuffer msg1 kem_state
+    /\ message1_disjoint_to_lbuffer msg1 entropy_p
+    /\ disjoint kem_state entropy_p
+
+  )
+  (ensures fun h0 res h1 ->
+    match res with
+      | TypeEdhoc.CUnsupportedAlgorithmOrInvalidConfig -> (
+        modifies (loc entropy_p |+| loc msg1.c_i
+            |+| loc msg1.pk_x |+| loc is.eph_kem_priv_key.value
+            |+| loc kem_state
+            |+| loc is.eph_kem_priv_key.is_some
+            |+| loc msg1.ct_auth_R |+| loc hs.k_auth_R
+            |+| loc hs.th1
+            |+| loc hs.prk1e) h0 h1
+        
+      )
+      | TypeEdhoc.CSuccess -> (
+        True
+      )
+      | _ -> False
+  )
