src/kemedhoc/Impl.KEMEDHOC.Core.fst
@@ -1,0 +1,35 @@
+module Impl.KEMEDHOC.Core
+
+module B = LowStar.Buffer
+module ST = FStar.HyperStack.ST
+module HS = FStar.HyperStack
+module S = FStar.Seq
+module Seq = Lib.Sequence
+
+(*Specification modules*)
+module Spec = Spec.KEMEDHOC.Core
+friend Spec.KEMEDHOC.Core
+module SpecCrypto = Spec.KEMEDHOC.CryptoPrimitives
+
+(*Specification modules*)
+module SpecCrypto = Spec.KEMEDHOC.CryptoPrimitives
+module SpecSerdEdhoc = Spec.EDHOC.Serialization
+module SpecParser = Spec.KEMEDHOC.Parser
+
+module TypeEdhoc = TypeHelper.EDHOC
+
+#push-options "--z3rlimit 10"
+let init_handshake_state #kcs hs
+  = lbufferOpt_set_None hs.k_xy;
+  lbufferOpt_set_None hs.k_auth_I;
+  lbufferOpt_set_None hs.th2;
+  lbufferOpt_set_None hs.th3;
+  lbufferOpt_set_None hs.th4;
+  lbufferOpt_set_None hs.prk2e;
+  lbufferOpt_set_None hs.prk3e2m;
+  lbufferOpt_set_None hs.prk4e3m;
+  lbufferOpt_set_None hs.prk_out;
+  lbufferOpt_set_None hs.prk_exporter;
+  lbufferOpt_set_None hs.remote_id_cred
+
+#pop-options
