src/kemedhoc/Impl.KEMEDHOC.Core.fsti
@@ -1,0 +1,347 @@
+module Impl.KEMEDHOC.Core
+
+(*LowStar related modules*)
+open Lib.ByteBuffer
+open Lib.IntTypes
+open Lib.Buffer
+
+module B = LowStar.Buffer
+module ST = FStar.HyperStack.ST
+module HS = FStar.HyperStack
+module S = FStar.Seq
+module Seq = Lib.Sequence
+
+(*Specification modules*)
+module Spec = Spec.KEMEDHOC.Core
+module SpecCrypto = Spec.KEMEDHOC.CryptoPrimitives
+
+(*EDHOC utilities*)
+// open Impl.EDHOC.Utilities
+
+(*KEMEDHOC utilities*)
+open Impl.KEMEDHOC.Types
+open Impl.KEMEDHOC.CryptoPrimitives
+// open Impl.KEMEDHOC.KeySchedule
+open Impl.KEMEDHOC.Parser
+// open Impl.KEMEDHOC.Ciphertext
+// open Impl.KEMEDHOC.TranscriptHash
+open Spec.KEMEDHOC.Base.Definitions
+
+(*Specification modules*)
+module SpecCrypto = Spec.KEMEDHOC.CryptoPrimitives
+module SpecSerdEdhoc = Spec.EDHOC.Serialization
+module SpecParser = Spec.KEMEDHOC.Parser
+
+module TypeEdhoc = TypeHelper.EDHOC
+
+(*--------------------------- Utilities*)
+let kem_key_pair_m_live (#kcs: supportedKemCipherSuite)
+  (h: HS.mem) (kp: kem_key_pair_m kcs)
+  = match kp with
+    | pub_key, priv_key -> live h pub_key /\ live h priv_key
+
+let kem_key_pair_m_disjoint (#kcs: supportedKemCipherSuite)
+  (kp: kem_key_pair_m kcs)
+  = match kp with
+    | pub_key, priv_key -> disjoint pub_key priv_key
+
+let kem_key_pair_m_union (#kcs: supportedKemCipherSuite)
+  (kp: kem_key_pair_m kcs)
+  = match kp with
+    | pub_key, priv_key -> loc pub_key |+| loc priv_key
+
+let is_valid_kem_key_pair_m (#kcs: supportedKemCipherSuite)
+  (h: HS.mem) (kp: kem_key_pair_m kcs)
+  = kem_key_pair_m_live h kp /\ kem_key_pair_m_disjoint kp
+
+(*---------------------------- Common between parties*)
+
+/// -----------------
+/// Party state
+/// -----------------
+noeq type party_state_m (kcs: supportedKemCipherSuite) = {
+  suite: lbuffer uint8 1ul;
+  static_kem_kp: kem_key_pair_m kcs;
+  id_cred: id_cred_buffer;
+  // only Initiator needs the below ephemeral private key
+  eph_kem_priv_key: lbufferOpt (kem_priv_key_size_t kcs);
+  remote_static_kem_pub_key: kem_pub_key_buff kcs;
+  remote_id_cred: cred_buffer;
+}
+
+let party_state_live (#kcs: supportedKemCipherSuite) (h: HS.mem)
+  (ps: party_state_m kcs)
+  = live h ps.suite /\ kem_key_pair_m_live h ps.static_kem_kp
+    /\ live h ps.id_cred /\ lbufferOpt_live h ps.eph_kem_priv_key
+    /\ live h ps.remote_static_kem_pub_key /\ live h ps.remote_id_cred
+
+let party_state_disjoint (#kcs: supportedKemCipherSuite) (ps: party_state_m kcs)
+  = B.all_disjoint [loc ps.suite; kem_key_pair_m_union ps.static_kem_kp;
+      loc ps.id_cred; lbufferOpt_loc ps.eph_kem_priv_key;
+      loc ps.remote_static_kem_pub_key; loc ps.remote_id_cred]
+    /\ kem_key_pair_m_disjoint ps.static_kem_kp
+
+let party_state_union (#kcs: supportedKemCipherSuite)
+  (ps: party_state_m kcs)
+  = loc ps.suite |+| kem_key_pair_m_union ps.static_kem_kp
+    |+| loc ps.id_cred |+| lbufferOpt_loc ps.eph_kem_priv_key
+    |+| loc ps.remote_static_kem_pub_key |+| loc ps.remote_id_cred
+
+let party_state_disjoint_to_lbuffer (#t:buftype) (#a:Type0) (#kcs: supportedKemCipherSuite)
+  (ps: party_state_m kcs) (buf: buffer_t t a)
+  = disjoint buf ps.suite /\ disjoint buf ps.id_cred
+    /\ lbufferOpt_disjoint_to_lbuff ps.eph_kem_priv_key buf /\ disjoint buf ps.remote_static_kem_pub_key
+    /\ disjoint buf ps.remote_id_cred
+    /\ disjoint buf (fst ps.static_kem_kp) /\ disjoint buf (snd ps.static_kem_kp)
+
+let party_state_disjoint_to_msg1 (#kcs: supportedKemCipherSuite)
+  (ps: party_state_m kcs) (m1: message1 kcs)
+  = B.all_disjoint [loc ps.suite; loc (fst ps.static_kem_kp);
+      loc (snd ps.static_kem_kp);
+      loc ps.id_cred;
+      loc ps.eph_kem_priv_key.is_some; loc ps.eph_kem_priv_key.value;
+      loc ps.remote_static_kem_pub_key; loc ps.remote_id_cred;
+
+      loc m1.method; loc m1.suite_i; loc m1.pk_x;
+      loc m1.ct_auth_R; loc m1.c_i; loc m1.c1
+    ]
+
+let is_valid_party_state_m (#kcs: supportedKemCipherSuite)
+  (h: HS.mem) (ps: party_state_m kcs)
+  = let suite_label = SpecSerdEdhoc.bytes_to_nat (as_seq h ps.suite) in
+  
+  party_state_live h ps /\ party_state_disjoint ps
+  /\ suite_label = 9
+
+type valid_party_state_m (kcs: supportedKemCipherSuite) (h: HS.mem)
+  = ps:party_state_m kcs {is_valid_party_state_m h ps}
+
+let is_party_state_eph_est_m (#kcs: supportedKemCipherSuite)
+  (h: HS.mem) (ps: party_state_m kcs)
+  = is_valid_party_state_m h ps
+    /\ lbufferOpt_is_Some h ps.eph_kem_priv_key
+
+let party_state_m_eval (#kcs: supportedKemCipherSuite)
+  (h: HS.mem) (ps: valid_party_state_m kcs h)
+  : GTot (Spec.party_state #kcs)
+  = let suite_label = SpecSerdEdhoc.bytes_to_nat (as_seq h ps.suite) in 
+  {
+    Spec.suite = suite_label;
+    Spec.static_kem_kp = kem_key_pair_m_eval h ps.static_kem_kp;
+    Spec.id_cred = as_seq h ps.id_cred;
+    Spec.eph_kem_priv_key = eval_lbuffer_opt h ps.eph_kem_priv_key;
+    Spec.remote_static_kem_pub_key = as_seq h ps.remote_static_kem_pub_key;
+    Spec.remote_id_cred = as_seq h ps.remote_id_cred;
+  }
+
+let lemma_ps_m_eval_equiv (#kcs: supportedKemCipherSuite)
+  (h: HS.mem) (ps: party_state_m kcs)
+  : Lemma 
+  (requires is_valid_party_state_m h ps)
+  (ensures (
+    let ps_s = party_state_m_eval #kcs h ps in
+
+    Some? ps_s.eph_kem_priv_key <==> lbufferOpt_is_Some h ps.eph_kem_priv_key
+  ))
+  [SMTPat (party_state_m_eval #kcs h ps)]
+  = ()
+
+/// -----------------
+/// Handshake state
+/// -----------------
+noeq type handshake_state_m (kcs: supportedKemCipherSuite) = {
+  suite_i: lbuffer uint8 1ul;
+  msg1_hash: hash_out_buff kcs;
+  k_xy: lbufferOpt (kem_shared_secret_size_t kcs);
+  k_auth_R: kem_shared_secret_buff kcs;
+  k_auth_I: lbufferOpt (kem_shared_secret_size_t kcs);
+  th1: hash_out_buff kcs;
+  th2: lbufferOpt (hash_size_t kcs);
+  th3: lbufferOpt (hash_size_t kcs);
+  th4: lbufferOpt (hash_size_t kcs);
+  prk1e: hash_out_buff kcs;
+  prk2e: lbufferOpt (hash_size_t kcs);
+  prk3e2m: lbufferOpt (hash_size_t kcs);
+  prk4e3m: lbufferOpt (hash_size_t kcs);
+  prk_out: lbufferOpt (hash_size_t kcs);
+  prk_exporter: lbufferOpt (hash_size_t kcs);
+  // ID credential of the remote party
+  remote_id_cred: lbufferOpt (size SpecParser.cred_size);
+}
+
+let handshake_state_m_live (#kcs: supportedKemCipherSuite)
+  (h: HS.mem) (hs: handshake_state_m kcs)
+  = live h hs.suite_i /\ live h hs.msg1_hash
+    /\ lbufferOpt_live h hs.k_xy /\ live h hs.k_auth_R
+    /\ lbufferOpt_live h hs.k_auth_I /\ live h hs.th1
+    /\ lbufferOpt_live h hs.th2 /\ lbufferOpt_live h hs.th3
+    /\ lbufferOpt_live h hs.th4 /\ live h hs.prk1e
+    /\ lbufferOpt_live h hs.prk2e /\ lbufferOpt_live h hs.prk3e2m
+    /\ lbufferOpt_live h hs.prk4e3m /\ lbufferOpt_live h hs.prk_out
+    /\ lbufferOpt_live h hs.prk_exporter
+    /\ lbufferOpt_live h hs.remote_id_cred
+
+let handshake_state_m_disjoint (#kcs: supportedKemCipherSuite)
+  (h: HS.mem) (hs: handshake_state_m kcs)
+  = B.all_disjoint [loc hs.suite_i; loc hs.msg1_hash;
+      loc hs.k_xy.is_some; loc hs.k_xy.value;
+      loc hs.k_auth_R;
+      loc hs.k_auth_I.is_some; loc hs.k_auth_I.value;
+      loc hs.th1;
+      loc hs.th2.is_some; loc hs.th2.value;
+      loc hs.th3.is_some; loc hs.th3.value;
+      loc hs.th4.is_some; loc hs.th4.value;
+      loc hs.prk1e; loc hs.prk2e.is_some; loc hs.prk2e.value;
+      loc hs.prk3e2m.is_some; loc hs.prk3e2m.value;
+      loc hs.prk4e3m.is_some; loc hs.prk4e3m.value;
+      loc hs.prk_out.is_some; loc hs.prk_out.value;
+      loc hs.prk_exporter.is_some; loc hs.prk_exporter.value;
+      loc hs.remote_id_cred.is_some; loc hs.remote_id_cred.value]
+
+let is_valid_handshake_state_m (#kcs: supportedKemCipherSuite)
+  (h: HS.mem) (hs: handshake_state_m kcs)
+  = let suite_label = SpecSerdEdhoc.bytes_to_nat (as_seq h hs.suite_i) in
+  handshake_state_m_live h hs /\ handshake_state_m_disjoint h hs
+  /\ suite_label = 9
+
+inline_for_extraction
+type valid_handshake_state_m (kcs: supportedKemCipherSuite) (h: HS.mem)
+  = hs:handshake_state_m kcs {is_valid_handshake_state_m h hs}
+
+let handshake_state_m_union (#kcs: supportedKemCipherSuite)
+  (hs: handshake_state_m kcs)
+  = loc hs.suite_i |+| loc hs.msg1_hash
+    |+| lbufferOpt_loc hs.k_xy |+| loc hs.k_auth_R
+    |+| lbufferOpt_loc hs.k_auth_I |+| loc hs.th1
+    |+| lbufferOpt_loc hs.th2 |+| lbufferOpt_loc hs.th3
+    |+| lbufferOpt_loc hs.th4 |+| loc hs.prk1e
+    |+| lbufferOpt_loc hs.prk2e |+| lbufferOpt_loc hs.prk3e2m
+    |+| lbufferOpt_loc hs.prk4e3m |+| lbufferOpt_loc hs.prk_out
+    |+| lbufferOpt_loc hs.prk_exporter
+    |+| lbufferOpt_loc hs.remote_id_cred
+
+let handshake_state_m_disjoint_to_lbuffer (#t:buftype) (#a:Type0) (#kcs: supportedKemCipherSuite)
+  (hs: handshake_state_m kcs) (buf: buffer_t t a)
+  = disjoint buf hs.suite_i /\ disjoint buf hs.msg1_hash
+    /\ lbufferOpt_disjoint_to_lbuff hs.k_xy buf
+    /\ disjoint buf hs.k_auth_R
+    /\ lbufferOpt_disjoint_to_lbuff hs.k_auth_I buf /\ disjoint buf hs.th1
+    /\ lbufferOpt_disjoint_to_lbuff hs.th2 buf
+    /\ lbufferOpt_disjoint_to_lbuff hs.th3 buf
+    /\ lbufferOpt_disjoint_to_lbuff hs.th4 buf /\ disjoint buf hs.prk1e
+    /\ lbufferOpt_disjoint_to_lbuff hs.prk2e buf
+    /\ lbufferOpt_disjoint_to_lbuff hs.prk3e2m buf
+    /\ lbufferOpt_disjoint_to_lbuff hs.prk4e3m buf
+    /\ lbufferOpt_disjoint_to_lbuff hs.prk_out buf
+    /\ lbufferOpt_disjoint_to_lbuff hs.prk_exporter buf
+    /\ lbufferOpt_disjoint_to_lbuff hs.remote_id_cred buf
+
+let handshake_state_m_disjoint_to_party_state (#kcs: supportedKemCipherSuite)
+  (hs: handshake_state_m kcs) (ps: party_state_m kcs)
+  = B.all_disjoint [loc hs.suite_i; loc hs.msg1_hash;
+      loc hs.k_xy.is_some; loc hs.k_xy.value;
+      loc hs.k_auth_R;
+      loc hs.k_auth_I.is_some; loc hs.k_auth_I.value;
+      loc hs.th1;
+      loc hs.th2.is_some; loc hs.th2.value;
+      loc hs.th3.is_some; loc hs.th3.value;
+      loc hs.th4.is_some; loc hs.th4.value;
+      loc hs.prk1e;
+      loc hs.prk2e.is_some; loc hs.prk2e.value;
+      loc hs.prk3e2m.is_some; loc hs.prk3e2m.value;
+      loc hs.prk4e3m.is_some; loc hs.prk4e3m.value;
+      loc hs.prk_out.is_some; loc hs.prk_out.value;
+      loc hs.prk_exporter.is_some; loc hs.prk_exporter.value;
+      loc hs.remote_id_cred.is_some; loc hs.remote_id_cred.value;
+
+      loc ps.suite; kem_key_pair_m_union ps.static_kem_kp;
+      loc ps.id_cred;
+      loc ps.eph_kem_priv_key.is_some; loc ps.eph_kem_priv_key.value;
+      loc ps.remote_static_kem_pub_key; loc ps.remote_id_cred
+    ]
+
+let handshake_state_m_disjoint_to_msg1 (#kcs: supportedKemCipherSuite)
+  (hs: handshake_state_m kcs) (m1: message1 kcs)
+  = B.all_disjoint [loc hs.suite_i; loc hs.msg1_hash;
+      loc hs.k_xy.is_some; loc hs.k_xy.value;
+      loc hs.k_auth_R;
+      loc hs.k_auth_I.is_some; loc hs.k_auth_I.value;
+      loc hs.th1;
+      loc hs.th2.is_some; loc hs.th2.value;
+      loc hs.th3.is_some; loc hs.th3.value;
+      loc hs.th4.is_some; loc hs.th4.value;
+      loc hs.prk1e;
+      loc hs.prk2e.is_some; loc hs.prk2e.value;
+      loc hs.prk3e2m.is_some; loc hs.prk3e2m.value;
+      loc hs.prk4e3m.is_some; loc hs.prk4e3m.value;
+      loc hs.prk_out.is_some; loc hs.prk4e3m.value;
+      loc hs.prk_exporter.is_some; loc hs.prk_exporter.value;
+      loc hs.remote_id_cred.is_some; loc hs.remote_id_cred.value;
+
+      loc m1.method; loc m1.suite_i; loc m1.pk_x;
+      loc m1.ct_auth_R; loc m1.c_i; loc m1.c1
+    ]
+
+let handshake_state_m_eval (#kcs: supportedKemCipherSuite)
+  (h: HS.mem) (hs: valid_handshake_state_m kcs h)
+  : GTot (Spec.handshake_state #kcs)
+  = let suite_label = SpecSerdEdhoc.bytes_to_nat (as_seq h hs.suite_i) in
+  {
+    Spec.suite_i = suite_label;
+    Spec.msg1_hash = as_seq h hs.msg1_hash;
+    Spec.k_xy = eval_lbuffer_opt h hs.k_xy;
+    Spec.k_auth_R = as_seq h hs.k_auth_R;
+    Spec.k_auth_I = eval_lbuffer_opt h hs.k_auth_I;
+    Spec.th1 = as_seq h hs.th1;
+    Spec.th2 = eval_lbuffer_opt h hs.th2;
+    Spec.th3 = eval_lbuffer_opt h hs.th3;
+    Spec.th4 = eval_lbuffer_opt h hs.th4;
+    Spec.prk1e = as_seq h hs.prk1e;
+    Spec.prk2e = eval_lbuffer_opt h hs.prk2e;
+    Spec.prk3e2m = eval_lbuffer_opt h hs.prk3e2m;
+    Spec.prk4e3m = eval_lbuffer_opt h hs.prk4e3m;
+    Spec.prk_out = eval_lbuffer_opt h hs.prk_out;
+    Spec.prk_exporter = eval_lbuffer_opt h hs.prk_exporter;
+    Spec.remote_id_cred = eval_lbuffer_opt h hs.remote_id_cred;
+  }
+
+/// Refined types for handshake state during the protocol run
+
+let is_hanbshake_state_m_after_init (#kcs: supportedKemCipherSuite)
+  (h: HS.mem) (hs: handshake_state_m kcs)
+  = is_valid_handshake_state_m h hs
+  /\ lbufferOpt_is_None h hs.k_xy
+    /\ lbufferOpt_is_None h hs.k_auth_I
+    /\ lbufferOpt_is_None h hs.th2
+    /\ lbufferOpt_is_None h hs.th3
+    /\ lbufferOpt_is_None h hs.th4
+    /\ lbufferOpt_is_None h hs.prk2e
+    /\ lbufferOpt_is_None h hs.prk3e2m
+    /\ lbufferOpt_is_None h hs.prk4e3m
+    /\ lbufferOpt_is_None h hs.prk_out
+    /\ lbufferOpt_is_None h hs.prk_exporter
+    /\ lbufferOpt_is_None h hs.remote_id_cred
+
+let modified_loc_hs_after_init (#kcs: supportedKemCipherSuite)
+  (hs: handshake_state_m kcs)
+  = loc hs.k_xy.is_some |+| loc hs.k_auth_I.is_some
+    |+| loc hs.th2.is_some |+| loc hs.th3.is_some |+| loc hs.th4.is_some
+    |+| loc hs.prk2e.is_some |+| loc hs.prk3e2m.is_some |+| loc hs.prk4e3m.is_some
+    |+| loc hs.prk_out.is_some |+| loc hs.prk_exporter.is_some
+    |+| loc hs.remote_id_cred.is_some
+
+val init_handshake_state:
+  #kcs: supportedKemCipherSuite
+  -> hs: handshake_state_m kcs
+  -> ST.Stack unit
+  (requires fun h0 ->
+    is_valid_handshake_state_m h0 hs
+  )
+  (ensures fun h0 _ h1 ->
+    let hs_s = Spec.init_handshake_state #kcs (as_seq h0 hs.msg1_hash)
+                (as_seq h0 hs.th1) (as_seq h0 hs.k_auth_R) (as_seq h0 hs.prk1e) in
+
+    modifies (modified_loc_hs_after_init hs) h0 h1
+    /\ is_hanbshake_state_m_after_init h1 hs
+    /\ Spec.hs_equal (handshake_state_m_eval h1 hs) hs_s
+  )
